Test/dafny0/Strings.dfy
@@ -87,6 +87,8 @@ method Main()
   // Ensuring we're precise enough about identifying \u escapes
   print "I'm afraid you'll find escape quite impossible, \\u007", "\n";
   print "Luckily I have this nifty gadget from my good friend, \\\u0051", "\n";
+
+  AllCharsTest();
 }
 
 method GimmieAChar(s: string) returns (ch: char)
@@ -135,3 +137,18 @@ method WeirdChars() returns (c: char, d: char)
   c := '\uD800';
   d := 0xDFFF as char;
 }
+
+method AllCharsTest() {
+  var allChars := set c: char {:trigger Identity(c)} | true :: Identity(c);
+  var allUTF16CodeUnits := set cp: int {:trigger Identity(cp)} | 0 <= cp < 0x1_0000 :: Identity(cp as char);
+  assert forall c: char {:trigger Identity(c)} :: 0 <= Identity(c as int) < 0x1_0000;
+  assert forall c: char :: Identity(c) in allChars;
+  assert allChars == allUTF16CodeUnits;
+
+  // I'd love to expect allChars == allCodePoints, but that's currently
+  // an O(n^2) operation in some runtimes that don't have hashcode-based
+  // set operations, and n here is 2^16. :P
+  expect |allChars| == |allUTF16CodeUnits|;
+}
+
+function method Identity<T>(x: T): T { x }
